Changing some files location

Deque/core.v
@@ -1,6 +1,7 @@
-From Coq Require Import Program List Arith Lia.
+From Coq Require Import Program List.
 Import ListNotations.
 From Equations Require Import Equations.
+Require Import Coq.Program.Equality.
 From Hammer Require Import Tactics.
 From AAC_tactics Require Import AAC.
 From AAC_tactics Require Import Instances.
@@ -12,48 +13,22 @@ From Color Require Import GYR.
 (* |                                 Types                                  | *)
 (* +------------------------------------------------------------------------+ *)
 
-(* A type for products. *)
-Inductive prodN (A : Type) : nat -> Type :=
-  | prodZ : A -> prodN A 0
-  | prodS {n : nat} : prodN A n -> prodN A n -> prodN A (S n).
-Arguments prodZ {A}.
-Arguments prodS {A n}.
-
-(* A type for options. *)
-Inductive optionN (A : Type) (lvl : nat) : nat -> Type :=
-  | NoneN : optionN A lvl 0
-  | SomeN : prodN A lvl -> optionN A lvl 1.
-Arguments NoneN {A lvl}.
-Arguments SomeN {A lvl}.
-
 (* A type for buffers. *)
-Inductive buffer (A : Type) (lvl : nat) : nat -> color -> Type :=
-  | B0         : buffer A lvl 0 red
-  | B1 {y r}   : prodN A lvl -> buffer A lvl 1 (Mix NoGreen y r)
-  | B2 {g y r} : prodN A lvl -> prodN A lvl -> buffer A lvl 2 (Mix g y r)
-  | B3 {g y r} : prodN A lvl -> prodN A lvl -> prodN A lvl ->
-                 buffer A lvl 3 (Mix g y r)
-  | B4 {y r}   : prodN A lvl -> prodN A lvl -> prodN A lvl ->
-                 prodN A lvl -> buffer A lvl 4 (Mix NoGreen y r)
-  | B5         : prodN A lvl -> prodN A lvl -> prodN A lvl ->
-                 prodN A lvl -> prodN A lvl -> buffer A lvl 5 red.
-Arguments B0 {A lvl}.
-Arguments B1 {A lvl y r}.
-Arguments B2 {A lvl g y r}.
-Arguments B3 {A lvl g y r}.
-Arguments B4 {A lvl y r}.
-Arguments B5 {A lvl}.
+Inductive buffer : Type -> color -> Type :=
+  | B0 {A}       :                          buffer A red
+  | B1 {A y r}   : A                     -> buffer A (Mix NoGreen y r)
+  | B2 {A g y r} : A -> A                -> buffer A (Mix g y r)
+  | B3 {A g y r} : A -> A -> A           -> buffer A (Mix g y r)
+  | B4 {A y r}   : A -> A -> A -> A      -> buffer A (Mix NoGreen y r)
+  | B5 {A}       : A -> A -> A -> A -> A -> buffer A red.
 
 (* A type for packets. *)
-Inductive packet (A : Type) (lvl : nat) : nat -> nat -> nat -> color -> Type :=
-  | Hole {size : nat} : packet A lvl lvl size size uncolored
-  | Packet {hlvl psize pktsize ssize hsize C y} :
-      buffer A lvl psize C ->
-      packet A (S lvl) hlvl pktsize hsize (Mix NoGreen y NoRed) ->
-      buffer A lvl ssize C ->
-      packet A lvl hlvl (psize + pktsize + pktsize + ssize) hsize C.
-Arguments Hole {A lvl size}.
-Arguments Packet {A lvl hlvl psize pktsize ssize hsize C y}.
+Inductive packet : Type -> Type -> color -> Type :=
+  | Hole {A} : packet A A uncolored
+  | Packet {A B C y} : buffer A C ->
+                       packet (A * A) B (Mix NoGreen y NoRed) ->
+                       buffer A C ->
+                       packet A B C.
 
 (* A type for the regularity relation. *)
 Inductive regularity : color -> color -> Type :=
@@ -62,45 +37,30 @@ Inductive regularity : color -> color -> Type :=
   | R       : regularity red    green.
 
 (* A type for chains. *)
-Inductive chain (A : Type) (lvl : nat) : nat -> color -> Type :=
-  | Ending {size : nat} {C : color} :
-      buffer A lvl size C ->
-      chain A lvl size green
-  | Chain {hlvl size hsize : nat} {C1 C2 : color} :
-      regularity C1 C2 ->
-      packet A lvl hlvl size hsize C1 ->
-      chain A hlvl hsize C2 ->
-      chain A lvl size C1.
-Arguments Ending {A lvl size C}.
-Arguments Chain {A lvl hlvl size hsize C1 C2}.
+Inductive chain : Type -> color -> Type :=
+  | Ending {A} : buffer A red -> chain A green
+  | Chain {A B C1 C2} :
+      regularity C1 C2 -> packet A B C1 -> chain B C2 -> chain A C1.
 
 (* A type decomposing buffers according to their number of elements.
    Buffers with 0 or 1 element are decomposed into [Underflow];
    buffers with 2 or 3 elements are decomposed into [Ok];
    buffers with 4 or 5 elements are decomposed into [Overflow]. *)
-Inductive decompose (A : Type) (lvl : nat) : nat -> Type :=
-  | Underflow {size : nat} : optionN A lvl size -> decompose A lvl size
-  | Ok {size : nat} : buffer A lvl size green -> decompose A lvl size
-  | Overflow {size : nat} :
-    buffer A lvl size green -> prodN A (S lvl) -> decompose A lvl (S (S size)).
-Arguments Underflow {A lvl size}.
-Arguments Ok {A lvl size}.
-Arguments Overflow {A lvl size}.
+Inductive decompose : Type -> Type :=
+  | Underflow {A} : option A -> decompose A
+  | Ok {A} : buffer A green -> decompose A
+  | Overflow {A} : buffer A green -> A * A -> decompose A.
 
 (* A type decomposing a buffer into its first element, a central buffer, and
    its last element. If such a decomposition is not possible, an option
    representing the buffer is returned with [Alone]. *)
-Inductive sandwich (A : Type) (lvl : nat) : nat -> Type :=
-  | Alone {s : nat} : optionN A lvl s -> sandwich A lvl s
-  | Sandwich {s : nat} {C : color} :
-    prodN A lvl -> buffer A lvl s C -> prodN A lvl -> sandwich A lvl (2 + s).
-Arguments Alone {A lvl s}.
-Arguments Sandwich {A lvl s C}.
+Inductive sandwich : Type -> Type :=
+  | Alone {A} : option A -> sandwich A
+  | Sandwich {A} : A -> buffer A red -> A -> sandwich A.
 
-(* A type for deque. *)
-Inductive deque (A : Type) (size : nat) : Type :=
-  | T {g y} : chain A 0 size (Mix g y NoRed) -> deque A size.
-Arguments T {A size g y}.
+(* A type for deques. *)
+Inductive deque : Type -> Type :=
+  | T {A g y} : chain A (Mix g y NoRed) -> deque A.
 
 (* +------------------------------------------------------------------------+ *)
 (* |                                 Models                                 | *)
@@ -114,227 +74,75 @@ Opaque app.
 Definition singleton {A : Type} (x : A) : list A := [x].
 Opaque singleton.
 
-(* A hint database of rewrites to be used when trying to automatically resolve
-   obligations on lists generated by [Equations]. *)
-#[export] Hint Rewrite <-app_assoc : rlist.
-#[export] Hint Rewrite app_nil_r : rlist.
-#[export] Hint Rewrite map_app : rlist.
-#[export] Hint Rewrite concat_app : rlist.
-
-(* In the following, [concat_map_***_seq] functions assume the structure [***]
-   contains elements of type [T A lvl] where [T : Type -> nat -> Type],
-   [A : Type] and [lvl : nat].
-
-   These functions are needed for the implementation of catenable deques. In
-   this implementation, non-catenable deques contain elements of type
-   [T A lvl] where [T] is instanciated with [stored_triple].
-
-   Such functions compute the sequence associated to the [***] structure, then
-   perform a map on them using the model functions [f] of the type [T], and
-   finally concatenate the resulting sequence to obtain a term of type [list A].
-
-   The model function for the [***] structure is just a special case of the
-   [concat_map_***_seq] function, where [T] is instanciated with [fun A _ => A]
-   and [f] is the singleton function.
-
-   The correct behavior of [concat_map_***_seq] functions is verified with
-   [correct_concat_map_***_seq] lemmas. *)
-
-(* Sequence + map + concat for products. *)
-Definition concat_map_prodN_seq
-  {T : Type -> nat -> Type}
-  (f : forall A lvl, T A lvl -> list A)
-  {A lvlt lvl} : prodN (T A lvlt) lvl -> list A :=
-  let fix local {lvl} (p : prodN (T A lvlt) lvl) : list A :=
-    match p with
-    | prodZ ta => f A lvlt ta
-    | prodS p1 p2 => local p1 ++ local p2
-    end
-  in local.
-
-(* Returns the sequence associated to a product. *)
-Notation prodN_seq :=
-  (concat_map_prodN_seq (T := fun A _ => A) (fun A _ a => [a]) (lvlt := 0)).
-
-(* Ensures the correct behavior of products model functions. *)
-Lemma correct_concat_map_prodN_seq
-  {T : Type -> nat -> Type}
-  (f : forall A lvl, T A lvl -> list A)
-  {A lvlt lvl} (p : prodN (T A lvlt) lvl) :
-  concat_map_prodN_seq f p = concat (map (f A lvlt) (prodN_seq p)).
-Proof.
-  induction p; hauto db:rlist.
-Qed.
+(* Returns the sequence associated to a pair. *)
+Equations pair_seq {A} : A * A -> list A :=
+pair_seq (a, b) := [a] ++ [b].
 
 (* Returns the sequence associated to an option. *)
-Equations optionN_seq {A lvl s} : optionN A lvl s -> list A :=
-optionN_seq NoneN := [];
-optionN_seq (SomeN x) := prodN_seq x.
-
-(* Sequence + map + concat for buffers. *)
-Definition concat_map_buffer_seq
-  {T : Type -> nat -> Type}
-  (f : forall A lvl, T A lvl -> list A)
-  {A lvlt lvl size C} (b : buffer (T A lvlt) lvl size C) : list A :=
-  match b with
-  | B0 => []
-  | (B1 a) => concat_map_prodN_seq f a
-  | (B2 a b) => concat_map_prodN_seq f a ++ concat_map_prodN_seq f b
-  | (B3 a b c) => concat_map_prodN_seq f a ++ concat_map_prodN_seq f b ++
-                  concat_map_prodN_seq f c
-  | (B4 a b c d) => concat_map_prodN_seq f a ++ concat_map_prodN_seq f b ++
-                    concat_map_prodN_seq f c ++ concat_map_prodN_seq f d
-  | (B5 a b c d e) => concat_map_prodN_seq f a ++ concat_map_prodN_seq f b ++
-                      concat_map_prodN_seq f c ++ concat_map_prodN_seq f d ++
-                      concat_map_prodN_seq f e
-  end.
+Equations option_seq {A} : option A -> list A :=
+option_seq None := [];
+option_seq (Some x) := [x].
 
 (* Returns the sequence associated to a buffer. *)
-Notation buffer_seq :=
-  (concat_map_buffer_seq (T := fun A _ => A) (fun A _ a => [a]) (lvlt := 0)).
+Equations buffer_seq {A C} : buffer A C -> list A :=
+buffer_seq B0 := [];
+buffer_seq (B1 a) := [a];
+buffer_seq (B2 a b) := [a] ++ [b];
+buffer_seq (B3 a b c) := [a] ++ [b] ++ [c];
+buffer_seq (B4 a b c d) := [a] ++ [b] ++ [c] ++ [d];
+buffer_seq (B5 a b c d e) := [a] ++ [b] ++ [c] ++ [d] ++ [e].
 
-(* Ensures the correct behavior of buffers model functions. *)
-Lemma correct_concat_map_buffer_seq
-  {T : Type -> nat -> Type}
-  (f : forall A lvl, T A lvl -> list A)
-  {A lvlt lvl size C} (b : buffer (T A lvlt) lvl size C) :
-  concat_map_buffer_seq f b = concat (map (f A lvlt) (buffer_seq b)).
+(* Transforms a list of pairs into a list of basic elements, while preserving
+   the order of elements. *)
+Equations flattenp {A} : list (A * A) -> list A :=
+flattenp [] := [];
+flattenp (p :: l) := pair_seq p ++ flattenp l.
+
+(* Proves that [flattenp] is distributive over [app]. *)
+Lemma flattenp_app [A] (l1 l2 : list (A * A)) :
+  flattenp (l1 ++ l2) = flattenp l1 ++ flattenp l2.
 Proof.
-  destruct b as [ | ?? a | ??? a b |  ??? a b c | ?? a b c d | a b c d e ];
-  simpl;
-  autorewrite with rlist.
-  - reflexivity.
-  - rewrite (correct_concat_map_prodN_seq _ a).
-    reflexivity.
-  - rewrite (correct_concat_map_prodN_seq _ a).
-    rewrite (correct_concat_map_prodN_seq _ b).
-    reflexivity.
-  - rewrite (correct_concat_map_prodN_seq _ a).
-    rewrite (correct_concat_map_prodN_seq _ b).
-    rewrite (correct_concat_map_prodN_seq _ c).
-    reflexivity.
-  - rewrite (correct_concat_map_prodN_seq _ a).
-    rewrite (correct_concat_map_prodN_seq _ b).
-    rewrite (correct_concat_map_prodN_seq _ c).
-    rewrite (correct_concat_map_prodN_seq _ d).
-    reflexivity.
-  - rewrite (correct_concat_map_prodN_seq _ a).
-    rewrite (correct_concat_map_prodN_seq _ b).
-    rewrite (correct_concat_map_prodN_seq _ c).
-    rewrite (correct_concat_map_prodN_seq _ d).
-    rewrite (correct_concat_map_prodN_seq _ e).
-    reflexivity.
+  revert l2. induction l1; intro.
+  - hauto.
+  - rewrite <-app_comm_cons.
+    hauto.
 Qed.
 
-(* Sequence + map + concat for packets. *)
-Definition concat_map_packet_seq
-  {T : Type -> nat -> Type}
-  (f : forall A lvl, T A lvl -> list A)
-  {A lvlt lvl hlvl pktsize hsize C} :
-  packet (T A lvlt) lvl hlvl pktsize hsize C -> list A -> list A :=
-  let fix local {lvl hlvl pktsize hsize C}
-    (pkt : packet (T A lvlt) lvl hlvl pktsize hsize C) (l : list A) : list A :=
-    match pkt with
-    | Hole => l
-    | Packet p pkt s => concat_map_buffer_seq f p ++
-                        local pkt l ++
-                        concat_map_buffer_seq f s
-    end
-  in local.
-
-(* Returns the sequence associated to a packet. *)
-Notation packet_seq :=
-  (concat_map_packet_seq (T := fun A _ => A) (fun A _ a => [a]) (lvlt := 0)).
-
-(* Ensures the correct behavior of packets model functions. *)
-Lemma correct_concat_map_packet_seq
-  {T : Type -> nat -> Type}
-  (f : forall A lvl, T A lvl -> list A)
-  {A lvlt lvl hlvl pktsize hsize C}
-  (pkt : packet (T A lvlt) lvl hlvl pktsize hsize C) (l : list (T A lvlt)) :
-  concat_map_packet_seq f pkt (concat (map (f A lvlt) l)) =
-    concat (map (f A lvlt) (packet_seq pkt l)).
-Proof.
-  induction pkt as [ | ???????? p pkt IHpkt s ]; simpl.
-  - reflexivity.
-  - autorewrite with rlist.
-    rewrite (correct_concat_map_buffer_seq _ p).
-    rewrite IHpkt.
-    rewrite (correct_concat_map_buffer_seq _ s).
-    reflexivity.
-Qed.
-
-(* Sequence + map + concat for chains. *)
-Definition concat_map_chain_seq
-  {T : Type -> nat -> Type}
-  (f : forall A lvl, T A lvl -> list A)
-  {A lvlt lvl size C} : chain (T A lvlt) lvl size C -> list A :=
-  let fix local {lvl size C} (c : chain (T A lvlt) lvl size C) : list A :=
-    match c with
-    | Ending b => concat_map_buffer_seq f b
-    | Chain _ pkt c => concat_map_packet_seq f pkt (local c)
-    end
-  in local.
+(* Returns the sequence associated to a packet, provided the sequence
+   associated to its hole. *)
+Equations packet_seq {A B C} : packet A B C -> list B -> list A :=
+packet_seq Hole l := l;
+packet_seq (Packet p pkt s) l :=
+  buffer_seq p ++ flattenp (packet_seq pkt l) ++ buffer_seq s.
 
 (* Returns the sequence associated to a chain. *)
-Notation chain_seq :=
-  (concat_map_chain_seq (T := fun A _ => A) (fun A _ a => [a]) (lvlt := 0)).
-
-(* Ensures the correct behavior of chains model functions. *)
-Lemma correct_concat_map_chain_seq
-  {T : Type -> nat -> Type}
-  (f : forall A lvl, T A lvl -> list A)
-  {A lvlt lvl size C} (c : chain (T A lvlt) lvl size C) :
-  concat_map_chain_seq f c = concat (map (f A lvlt) (chain_seq c)).
-Proof.
-  induction c as [ b | ?????? reg pkt c ]; simpl.
-  - apply correct_concat_map_buffer_seq.
-  - rewrite IHc.
-    apply correct_concat_map_packet_seq.
-Qed.
+Equations chain_seq {A C} : chain A C -> list A :=
+chain_seq (Ending b) := buffer_seq b;
+chain_seq (Chain _ pkt c) := packet_seq pkt (chain_seq c).
 
 (* Returns the first 4 elements of the sequence associated to a decomposed
-   buffer.*)
-Equations decompose_main_seq {A lvl s} : decompose A lvl s -> list A :=
-decompose_main_seq (Underflow opt) := optionN_seq opt;
+   buffer. *)
+Equations decompose_main_seq {A : Type} : decompose A -> list A :=
+decompose_main_seq (Underflow o) := option_seq o;
 decompose_main_seq (Ok b) := buffer_seq b;
 decompose_main_seq (Overflow b _) := buffer_seq b.
 
 (* Returns the sequence associated to a decomposed buffer from the 5th element
    to the end  *)
-Equations decompose_rest_seq {A lvl s} : decompose A lvl s -> list A :=
+Equations decompose_rest_seq {A : Type} : decompose A -> list A :=
 decompose_rest_seq (Underflow _) := [];
 decompose_rest_seq (Ok _) := [];
-decompose_rest_seq (Overflow _ p) := prodN_seq p.
+decompose_rest_seq (Overflow _ (x, y)) := [x] ++ [y].
 
 (* Returns the sequence associated to a sandwiched buffer. *)
-Equations sandwich_seq {A lvl size} : sandwich A lvl size -> list A :=
-sandwich_seq (Alone opt) := optionN_seq opt;
-sandwich_seq (Sandwich x b y) := prodN_seq x ++ buffer_seq b ++ prodN_seq y.
-
-(* Sequence + map + concat for deques. *)
-Definition concat_map_deque_seq
-  {T : Type -> nat -> Type}
-  (f : forall A lvl, T A lvl -> list A)
-  {A lvlt size} (d : deque (T A lvlt) size) : list A :=
-  match d with
-  | T c => concat_map_chain_seq f c
-  end.
+Equations sandwich_seq {A : Type} : sandwich A -> list A :=
+sandwich_seq (Alone None) := [];
+sandwich_seq (Alone (Some x)) := [x];
+sandwich_seq (Sandwich x b y) := [x] ++ buffer_seq b ++ [y].
 
 (* Returns the sequence associated to a deque. *)
-Notation deque_seq :=
-  (concat_map_deque_seq (T := fun A _ => A) (fun A _ a => [a]) (lvlt := 0)).
-
-(* Ensures the correct behavior of deques model functions. *)
-Lemma correct_concat_map_deque_seq
-  {T : Type -> nat -> Type}
-  (f : forall A lvl, T A lvl -> list A)
-  {A lvlt size} (d : deque (T A lvlt) size) :
-  concat_map_deque_seq f d = concat (map (f A lvlt) (deque_seq d)).
-Proof.
-  destruct d.
-  apply correct_concat_map_chain_seq.
-Qed.
+Equations deque_seq {A} : deque A -> list A :=
+deque_seq (T c) := chain_seq c.
 
 Unset Equations Transparent.
 
@@ -345,116 +153,91 @@ Unset Equations Transparent.
 (* Notation for dependent types hiding the property on [x]. *)
 Notation "? x" := (@exist _ _ x _) (at level 100).
 
-(* Setting the default tactics for obligations to be [hauto] using the [rlist]
-   hint database. *)
-#[local] Obligation Tactic := try (cbn; hauto db:rlist).
-
-(* The empty deque. *)
-Equations empty {A} : { d : deque A 0 | deque_seq d = [] } :=
-empty := ? T (Ending B0).
-
 (* Pushes on a green buffer. *)
-Equations green_push {A lvl size}
-  (x : prodN A lvl) (b : buffer A lvl size green) :
-  { b' : buffer A lvl (S size) yellow |
-    buffer_seq b' = prodN_seq x ++ buffer_seq b } :=
+Equations green_push {A : Type} (x : A) (b : buffer A green) :
+  { b' : buffer A yellow | buffer_seq b' = [x] ++ buffer_seq b } :=
 green_push x (B2 a b)   := ? B3 x a b;
 green_push x (B3 a b c) := ? B4 x a b c.
 
 (* Injects on a green buffer. *)
-Equations green_inject {A lvl size}
-  (b : buffer A lvl size green) (x : prodN A lvl) :
-  { b' : buffer A lvl (S size) yellow |
-    buffer_seq b' = buffer_seq b ++ prodN_seq x } :=
+Equations green_inject {A : Type} (b : buffer A green) (x : A) :
+  { b' : buffer A yellow | buffer_seq b' = buffer_seq b ++ [x] } :=
 green_inject (B2 a b)   x := ? B3 a b x;
 green_inject (B3 a b c) x := ? B4 a b c x.
 
 (* Pops off a green buffer. *)
-Equations green_pop {A lvl size} (b : buffer A lvl size green) :
-  { '(x, b') : prodN A lvl * buffer A lvl (Nat.pred size) yellow |
-    buffer_seq b = prodN_seq x ++ buffer_seq b' } :=
+Equations green_pop {A : Type} (b : buffer A green) :
+  { '(x, b') : A * buffer A yellow | buffer_seq b = [x] ++ buffer_seq b' } :=
 green_pop (B2 a b)   := ? (a, B1 b);
 green_pop (B3 a b c) := ? (a, B2 b c).
 
 (* Ejects off a green buffer. *)
-Equations green_eject {A lvl size} (b : buffer A lvl size green) :
-  { '(b', x) : buffer A lvl (Nat.pred size) yellow * prodN A lvl |
-    buffer_seq b = buffer_seq b' ++ prodN_seq x } :=
+Equations green_eject {A : Type} (b : buffer A green) :
+  { '(b', x) : buffer A yellow * A | buffer_seq b = buffer_seq b' ++ [x] } :=
 green_eject (B2 a b)   := ? (B1 a, b);
 green_eject (B3 a b c) := ? (B2 a b, c).
 
 (* Pushes on a yellow buffer. *)
-Equations yellow_push {A lvl size}
-  (x : prodN A lvl) (b : buffer A lvl size yellow) :
-  { b' : buffer A lvl (S size) red |
-    buffer_seq b' = prodN_seq x ++ buffer_seq b } :=
+Equations yellow_push {A : Type} (x : A) (b : buffer A yellow) :
+  { b' : buffer A red | buffer_seq b' = [x] ++ buffer_seq b } :=
 yellow_push x (B1 a)       := ? B2 x a;
 yellow_push x (B2 a b)     := ? B3 x a b;
 yellow_push x (B3 a b c)   := ? B4 x a b c;
 yellow_push x (B4 a b c d) := ? B5 x a b c d.
 
 (* Injects on a yellow buffer. *)
-Equations yellow_inject {A lvl size}
-  (b : buffer A lvl size yellow) (x : prodN A lvl) :
-  { b' : buffer A lvl (S size) red |
-    buffer_seq b' = buffer_seq b ++ prodN_seq x } :=
+Equations yellow_inject {A : Type} (b : buffer A yellow) (x : A) :
+  { b' : buffer A red | buffer_seq b' = buffer_seq b ++ [x] } :=
 yellow_inject (B1 a)       x := ? B2 a x;
 yellow_inject (B2 a b)     x := ? B3 a b x;
 yellow_inject (B3 a b c)   x := ? B4 a b c x;
 yellow_inject (B4 a b c d) x := ? B5 a b c d x.
 
 (* Pops off a yellow buffer. *)
-Equations yellow_pop {A lvl size} (b : buffer A lvl size yellow) :
-  { '(x, b') : prodN A lvl * buffer A lvl (Nat.pred size) red |
-    buffer_seq b = prodN_seq x ++ buffer_seq b' } :=
+Equations yellow_pop {A : Type} (b : buffer A yellow) :
+  { '(x, b') : A * buffer A red | buffer_seq b = [x] ++ buffer_seq b' } :=
 yellow_pop (B1 a)       := ? (a, B0);
 yellow_pop (B2 a b)     := ? (a, B1 b);
 yellow_pop (B3 a b c)   := ? (a, B2 b c);
 yellow_pop (B4 a b c d) := ? (a, B3 b c d).
 
 (* Ejects off a yellow buffer. *)
-Equations yellow_eject {A lvl size} (b : buffer A lvl size yellow) :
-  { '(b', x) : buffer A lvl (Nat.pred size) red * prodN A lvl |
-    buffer_seq b = buffer_seq b' ++ prodN_seq x } :=
+Equations yellow_eject {A : Type} (b : buffer A yellow) :
+  { '(b', x) : buffer A red * A | buffer_seq b = buffer_seq b' ++ [x] } :=
 yellow_eject (B1 a)       := ? (B0, a);
 yellow_eject (B2 a b)     := ? (B1 a, b);
 yellow_eject (B3 a b c)   := ? (B2 a b, c);
 yellow_eject (B4 a b c d) := ? (B3 a b c, d).
 
 (* Pushes on a buffer, and returns a green chain. *)
-Equations buffer_push {A lvl size C}
-  (x : prodN A lvl) (b : buffer A lvl size C) :
-  { c : chain A lvl (S size) green |
-    chain_seq c = prodN_seq x ++ buffer_seq b } :=
+Equations buffer_push {A C} (x : A) (b : buffer A C) :
+  { c : chain A green | chain_seq c = [x] ++ buffer_seq b } :=
 buffer_push x B0 := ? Ending (B1 x);
 buffer_push x (B1 a) := ? Ending (B2 x a);
 buffer_push x (B2 a b) := ? Ending (B3 x a b);
 buffer_push x (B3 a b c) := ? Ending (B4 x a b c);
 buffer_push x (B4 a b c d) := ? Ending (B5 x a b c d);
 buffer_push x (B5 a b c d e) :=
-  ? Chain G (Packet (B3 x a b) Hole (B3 c d e)) (Ending B0).
+    ? Chain G (Packet (B3 x a b) Hole (B3 c d e)) (Ending B0).
 
 (* Injects on a buffer, and returns a green chain. *)
-Equations buffer_inject {A lvl size C}
-  (b : buffer A lvl size C) (x : prodN A lvl) :
-  { c : chain A lvl (S size) green |
-    chain_seq c = buffer_seq b ++ prodN_seq x } :=
+Equations buffer_inject {A C} (b : buffer A C) (x : A) :
+  { c : chain A green | chain_seq c = buffer_seq b ++ [x] } :=
 buffer_inject B0 x := ? Ending (B1 x);
 buffer_inject (B1 a) x := ? Ending (B2 a x);
 buffer_inject (B2 a b) x := ? Ending (B3 a b x);
 buffer_inject (B3 a b c) x := ? Ending (B4 a b c x);
 buffer_inject (B4 a b c d) x := ? Ending (B5 a b c d x);
 buffer_inject (B5 a b c d e) x :=
-  ? Chain G (Packet (B3 a b c) Hole (B3 d e x)) (Ending B0).
+    ? Chain G (Packet (B3 a b c) Hole (B3 d e x)) (Ending B0).
 
-(* Pops off a buffer, and returns an option.
-   Extra properties about the size of the buffer are returned. *)
-Equations buffer_pop {A lvl size C} (b : buffer A lvl size C) :
-  { o : option (prodN A lvl * buffer A lvl (Nat.pred size) red) |
+(* Pops off a buffer, and returns an option. *)
+Equations buffer_pop {A C} (b : buffer A C) :
+  { o : option (A * buffer A red) |
+    buffer_seq b =
     match o with
-    | None => buffer_seq b = [] /\ size = 0
-    | Some (x, b') => buffer_seq b = prodN_seq x ++ buffer_seq b' /\
-                      exists s, size = S s
+    | None => []
+    | Some (x, b') => [x] ++ buffer_seq b'
     end } :=
 buffer_pop B0 := ? None;
 buffer_pop (B1 a) := ? Some (a, B0);
@@ -463,14 +246,13 @@ buffer_pop (B3 a b c) := ? Some (a, B2 b c);
 buffer_pop (B4 a b c d) := ? Some (a, B3 b c d);
 buffer_pop (B5 a b c d e) := ? Some (a, B4 b c d e).
 
-(* Ejects off a buffer, and returns an option.
-   Extra properties about the size of the buffer are returned. *)
-Equations buffer_eject {A lvl size C} (b : buffer A lvl size C) :
-  { o : option (buffer A lvl (Nat.pred size) red * prodN A lvl) |
+(* Ejects off a buffer, and returns an option. *)
+Equations buffer_eject {A C} (b : buffer A C) :
+  { o : option (buffer A red * A) |
+    buffer_seq b =
     match o with
-    | None => buffer_seq b = [] /\ size = 0
-    | Some (b', x) => buffer_seq b = buffer_seq b' ++ prodN_seq x /\
-                      exists s, size = S s
+    | None => []
+    | Some (b', x) => buffer_seq b' ++ [x]
     end } :=
 buffer_eject B0 := ? None;
 buffer_eject (B1 a) := ? Some (B0, a);
@@ -480,9 +262,8 @@ buffer_eject (B4 a b c d) := ? Some (B3 a b c, d);
 buffer_eject (B5 a b c d e) := ? Some (B4 a b c d, e).
 
 (* Pushes then ejects. *)
-Equations prefix_rot {A lvl size C} (x : prodN A lvl) (b : buffer A lvl size C) :
-  { '(b', y) : buffer A lvl size C * prodN A lvl |
-    prodN_seq x ++ buffer_seq b = buffer_seq b' ++ prodN_seq y } :=
+Equations prefix_rot {A C} (x : A) (b : buffer A C) :
+  { '(b', y) : buffer A C * A | [x] ++ buffer_seq b = buffer_seq b' ++ [y] } :=
 prefix_rot x B0 := ? (B0, x);
 prefix_rot x (B1 a) := ? (B1 x, a);
 prefix_rot x (B2 a b) := ? (B2 x a, b);
@@ -491,9 +272,8 @@ prefix_rot x (B4 a b c d) := ? (B4 x a b c, d);
 prefix_rot x (B5 a b c d e) := ? (B5 x a b c d, e).
 
 (* Injects then pops. *)
-Equations suffix_rot {A lvl size C} (b : buffer A lvl size C) (y : prodN A lvl) :
-  { '(x, b') : prodN A lvl * buffer A lvl size C |
-    buffer_seq b ++ prodN_seq y = prodN_seq x ++ buffer_seq b' } :=
+Equations suffix_rot {A C} (b : buffer A C) (y : A) :
+  { '(x, b') : A * buffer A C | buffer_seq b ++ [y] = [x] ++ buffer_seq b' } :=
 suffix_rot B0 x := ? (x, B0);
 suffix_rot (B1 a) x := ? (a, B1 x);
 suffix_rot (B2 a b) x := ? (a, B2 b x);
@@ -502,93 +282,85 @@ suffix_rot (B4 a b c d) x := ? (a, B4 b c d x);
 suffix_rot (B5 a b c d e) x := ? (a, B5 b c d e x).
 
 (* Merges an option and a pair to create a green buffer. *)
-Equations prefix23 {A lvl s} (o : optionN A lvl s) (p: prodN A (S lvl)) :
-  { b : buffer A lvl (2 + s) green |
-    buffer_seq b = optionN_seq o ++ prodN_seq p } :=
-prefix23  NoneN    (prodS b c) := ? B2 b c;
-prefix23 (SomeN a) (prodS b c) := ? B3 a b c.
+Equations prefix23 {A} (o : option A) (p: A * A) :
+  { b : buffer A green | buffer_seq b = option_seq o ++ pair_seq p } :=
+prefix23  None    (b, c) := ? B2 b c;
+prefix23 (Some a) (b, c) := ? B3 a b c.
 
 (* Merges a pair and an option to create a green buffer. *)
-Equations suffix23 {A lvl s} (p : prodN A (S lvl)) (o : optionN A lvl s) :
-  { b : buffer A lvl (2 + s) green |
-    buffer_seq b = prodN_seq p ++ optionN_seq o } :=
-suffix23 (prodS a b)  NoneN    := ? B2 a b;
-suffix23 (prodS a b) (SomeN c) := ? B3 a b c.
+Equations suffix23 {A} (p : A * A) (o : option A) :
+  { b : buffer A green | buffer_seq b = pair_seq p ++ option_seq o } :=
+suffix23 (a, b)  None    := ? B2 a b;
+suffix23 (a, b) (Some c) := ? B3 a b c.
 
 (* Merges an element and an option to create a yellow buffer. *)
-Equations suffix12 {A lvl s} (x : prodN A lvl) (o : optionN A lvl s) :
-  { b : buffer A lvl (S s) yellow |
-    buffer_seq b = prodN_seq x ++ optionN_seq o } :=
-suffix12 x  NoneN    := ? B1 x;
-suffix12 x (SomeN y) := ? B2 x y.
+Equations suffix12 {A} (x : A) (o : option A) :
+  { b : buffer A yellow | buffer_seq b = [x] ++ option_seq o } :=
+suffix12 x  None    := ? B1 x;
+suffix12 x (Some y) := ? B2 x y.
 
 (* Returns the decomposed version of a buffer. Here, it is a prefix
    decomposition: when the buffer has 4 or 5 elements, those at the end are
    set appart. *)
-Equations prefix_decompose {A lvl size C} (b : buffer A lvl size C) :
-  { dec : decompose A lvl size |
-    buffer_seq b = decompose_main_seq dec ++ decompose_rest_seq dec } :=
-prefix_decompose B0 := ? Underflow NoneN;
-prefix_decompose (B1 a) := ? Underflow (SomeN a);
+Equations prefix_decompose {A C} (b : buffer A C) :
+  { dec : decompose A | buffer_seq b = decompose_main_seq dec ++ decompose_rest_seq dec } :=
+prefix_decompose B0 := ? Underflow None;
+prefix_decompose (B1 a) := ? Underflow (Some a);
 prefix_decompose (B2 a b) := ? Ok (B2 a b);
 prefix_decompose (B3 a b c) := ? Ok (B3 a b c);
-prefix_decompose (B4 a b c d) := ? Overflow (B2 a b) (prodS c d);
-prefix_decompose (B5 a b c d e) := ? Overflow (B3 a b c) (prodS d e).
+prefix_decompose (B4 a b c d) := ? Overflow (B2 a b) (c, d);
+prefix_decompose (B5 a b c d e) := ? Overflow (B3 a b c) (d, e).
 
 (* Returns the decomposed version of a buffer. Here, it is a suffix
    decomposition: when the buffer has 4 or 5 elements, those at the start are
    set appart. *)
-Equations suffix_decompose {A lvl size C} (b : buffer A lvl size C) :
-  { dec : decompose A lvl size |
-    buffer_seq b = decompose_rest_seq dec ++ decompose_main_seq dec } :=
-suffix_decompose B0 := ? Underflow NoneN;
-suffix_decompose (B1 a) := ? Underflow (SomeN a);
+Equations suffix_decompose {A C} (b : buffer A C) :
+  { dec : decompose A | buffer_seq b = decompose_rest_seq dec ++ decompose_main_seq dec } :=
+suffix_decompose B0 := ? Underflow None;
+suffix_decompose (B1 a) := ? Underflow (Some a);
 suffix_decompose (B2 a b) := ? Ok (B2 a b);
 suffix_decompose (B3 a b c) := ? Ok (B3 a b c);
-suffix_decompose (B4 a b c d) := ? Overflow (B2 c d) (prodS a b);
-suffix_decompose (B5 a b c d e) := ? Overflow (B3 c d e) (prodS a b).
+suffix_decompose (B4 a b c d) := ? Overflow (B2 c d) (a, b);
+suffix_decompose (B5 a b c d e) := ? Overflow (B3 c d e) (a, b).
 
 (* Returns the sandwiched version of a buffer. *)
-Equations buffer_unsandwich {A lvl size C} (b : buffer A lvl size C) :
-  { sw : sandwich A lvl size | buffer_seq b = sandwich_seq sw } :=
-buffer_unsandwich B0 := ? Alone NoneN;
-buffer_unsandwich (B1 a) := ? Alone (SomeN a);
+Equations buffer_unsandwich {A C} (b : buffer A C) :
+  { sw : sandwich A | buffer_seq b = sandwich_seq sw } :=
+buffer_unsandwich B0 := ? Alone None;
+buffer_unsandwich (B1 a) := ? Alone (Some a);
 buffer_unsandwich (B2 a b) := ? Sandwich a B0 b;
 buffer_unsandwich (B3 a b c) := ? Sandwich a (B1 b) c;
 buffer_unsandwich (B4 a b c d) := ? Sandwich a (B2 b c) d;
 buffer_unsandwich (B5 a b c d e) := ? Sandwich a (B3 b c d) e.
 
-(* In the following, n-buffer denote a buffer of level n. *)
-
-(* Converts a n-buffer to a (n+1)-buffer. If the buffer has an odd number of
+(* Converts a buffer to a buffer of pairs. If the buffer has an odd number of
    elements, the first is returned via an option. *)
-Equations buffer_halve {A lvl size C} (b : buffer A lvl size C) :
-  { '(o, b') : optionN A lvl (size mod 2) * buffer A (S lvl) (size / 2) red |
-    buffer_seq b = optionN_seq o ++ buffer_seq b' } :=
-buffer_halve B0 := ? (NoneN, B0);
-buffer_halve (B1 a) := ? (SomeN a, B0);
-buffer_halve (B2 a b) := ? (NoneN, B1 (prodS a b));
-buffer_halve (B3 a b c) := ? (SomeN a, B1 (prodS b c));
-buffer_halve (B4 a b c d) := ? (NoneN, B2 (prodS a b) (prodS c d));
-buffer_halve (B5 a b c d e) := ? (SomeN a, B2 (prodS b c) (prodS d e)).
+Equations buffer_halve {A C} (b : buffer A C) :
+  { '(o, b') : option A * buffer (A * A) red |
+    buffer_seq b = option_seq o ++ flattenp (buffer_seq b') } :=
+buffer_halve B0 := ? (None, B0);
+buffer_halve (B1 a) := ? (Some a, B0);
+buffer_halve (B2 a b) := ? (None, B1 (a, b));
+buffer_halve (B3 a b c) := ? (Some a, B1 (b, c));
+buffer_halve (B4 a b c d) := ? (None, B2 (a, b) (c, d));
+buffer_halve (B5 a b c d e) := ? (Some a, B2 (b, c) (d, e)).
 
 (* Makes a non-red buffer yellow. *)
-Equations to_yellow {A lvl s g y} :
-  buffer A lvl s (Mix g y NoRed) -> buffer A lvl s yellow :=
+Equations to_yellow {A g y} : buffer A (Mix g y NoRed) -> buffer A yellow :=
 to_yellow (B1 a) := B1 a;
 to_yellow (B2 a b) := B2 a b;
 to_yellow (B3 a b c) := B3 a b c;
 to_yellow (B4 a b c d) := B4 a b c d.
 
 (* Proves the sequence of a buffer remains the same when it is made yellow. *)
-Lemma to_yellow_seq [A lvl size g y] (b : buffer A lvl size (Mix g y NoRed)) :
+Lemma to_yellow_seq [A g y] (b : buffer A (Mix g y NoRed)) :
   buffer_seq (to_yellow b) = buffer_seq b.
 Proof.
   dependent destruction b; reflexivity.
 Qed.
 
 (* Makes a buffer of any color red. *)
-Equations to_red {A lvl s C} : buffer A lvl s C -> buffer A lvl s red :=
+Equations to_red {A C} : buffer A C -> buffer A red :=
 to_red B0 := B0;
 to_red (B1 a) := B1 a;
 to_red (B2 a b) := B2 a b;
@@ -597,339 +369,228 @@ to_red (B4 a b c d) := B4 a b c d;
 to_red (B5 a b c d e) := B5 a b c d e.
 
 (* Proves the sequence of a buffer remains the same when it is made red. *)
-Lemma to_red_seq [A lvl size C] (b : buffer A lvl size C) :
+Lemma to_red_seq [A C] (b : buffer A C) :
   buffer_seq (to_red b) = buffer_seq b.
 Proof.
   destruct b; reflexivity.
 Qed.
 
-(* The last two lemmas are added to the hint database. *)
+(* A hint database of rewrites to be used when trying to automatically resolve
+   obligations generated by [Equations]. *)
+#[export] Hint Rewrite <-app_assoc : rlist.
+#[export] Hint Rewrite app_nil_r : rlist.
+#[export] Hint Rewrite flattenp_app : rlist.
 #[export] Hint Rewrite to_yellow_seq : rlist.
 #[export] Hint Rewrite to_red_seq : rlist.
 
-(* Takes a n-buffer of any color and a green (n+1)-buffer, rearranges elements
+(* Setting the default tactics for obligations to be [hauto] using the [rlist]
+   hint database. *)
+#[local] Obligation Tactic := try (cbn; hauto db:rlist).
+
+(* Takes a buffer of any color and a green buffer of pairs, rearranges elements
    contained in them, and returns a green buffer and a yellow buffer of pairs.
    The order of elements is preserved. *)
-Equations green_prefix_concat {A lvl size1 size2 C}
-  (b1 : buffer A lvl size1 C)
-  (b2 : buffer A (S lvl) size2 green) :
-  { '(b1', b2') : buffer A lvl (2 + size1 mod 2) green *
-                  buffer A (S lvl) (Nat.pred (size1 / 2 + size2)) yellow |
-    buffer_seq b1 ++ buffer_seq b2 =
-    buffer_seq b1' ++ buffer_seq b2' } :=
-green_prefix_concat B0 b2 with green_pop b2 => {
-  | ? (prodS a b, b3) := ? (B2 a b, b3) };
-green_prefix_concat (B1 a) b2 with green_pop b2 => {
-  | ? (prodS b c, b3) := ? (B3 a b c, b3) };
-green_prefix_concat (B2 a b) b2 := ? (B2 a b, to_yellow b2);
-green_prefix_concat (B3 a b c) b2 := ? (B3 a b c, to_yellow b2);
-green_prefix_concat (B4 a b c d) b2 with green_push (prodS c d) b2 => {
-  | ? b3 := ? (B2 a b, b3) };
-green_prefix_concat (B5 a b c d e) b2 with green_push (prodS d e) b2 => {
-  | ? b3 := ? (B3 a b c, b3) }.
+Equations green_prefix_concat {A C}
+  (b1 : buffer A C)
+  (b2 : buffer (A * A) green) :
+  { '(b1', b2') : buffer A green * buffer (A * A) yellow |
+    buffer_seq b1  ++ flattenp (buffer_seq b2) =
+    buffer_seq b1' ++ flattenp (buffer_seq b2') } :=
+green_prefix_concat b1 b2 with prefix_decompose b1 => {
+  | ? Underflow opt with green_pop b2 => {
+    | ? (ab, b) with prefix23 opt ab => {
+      | ? prefix := ? (prefix, b) } };
+  | ? Ok b := ? (b, to_yellow b2);
+  | ? Overflow b ab with green_push ab b2 => {
+    | ? suffix := ? (b, suffix) } }.
 
-(* Takes a green (n+1)-buffer and a n-buffer of any color, rearranges elements
+(* Takes a green buffer of pairs and a buffer of any color, rearranges elements
    contained in them, and returns a yellow buffer of pairs and a green buffer.
    The order of elements is preserved. *)
-Equations green_suffix_concat {A lvl size1 size2 C}
-  (b1 : buffer A (S lvl) size1 green)
-  (b2 : buffer A lvl size2 C) :
-  { '(b1', b2') : buffer A (S lvl) (Nat.pred (size2 / 2 + size1)) yellow *
-                  buffer A lvl (2 + size2 mod 2) green |
-    buffer_seq b1 ++ buffer_seq b2 =
-    buffer_seq b1' ++ buffer_seq b2' } :=
-green_suffix_concat b1 B0 with green_eject b1 => {
-  | ? (b3, prodS a b) := ? (b3, B2 a b) };
-green_suffix_concat b1 (B1 c) with green_eject b1 => {
-  | ? (b3, prodS a b) := ? (b3, B3 a b c) };
-green_suffix_concat b1 (B2 a b) := ? (to_yellow b1, B2 a b);
-green_suffix_concat b1 (B3 a b c) := ? (to_yellow b1, B3 a b c);
-green_suffix_concat b1 (B4 a b c d) with green_inject b1 (prodS a b) => {
-  | ? b3 := ? (b3, B2 c d) };
-green_suffix_concat b1 (B5 a b c d e) with green_inject b1 (prodS a b) => {
-  | ? b3 := ? (b3, B3 c d e) }.
+Equations green_suffix_concat {A C}
+  (b1 : buffer (A * A) green)
+  (b2 : buffer A C) :
+  { '(b1', b2') : buffer (A * A) yellow * buffer A green |
+    flattenp (buffer_seq b1)  ++ buffer_seq b2 =
+    flattenp (buffer_seq b1') ++ buffer_seq b2' } :=
+green_suffix_concat b1 b2 with suffix_decompose b2 => {
+  | ? Underflow opt with green_eject b1 => {
+    | ? (b, ab) with suffix23 ab opt => {
+      | ? suffix := ? (b, suffix) } };
+  | ? Ok b := ? (to_yellow b1, b);
+  | ? Overflow b ab with green_inject b1 ab => {
+    | ? prefix := ? (prefix, b) } }.
 
-(* Takes a n-buffer of any color and a yellow (n+1)-buffer, rearranges elements
-   contained in them, and returns a green buffer and a buffer of pairs of any
-   color.
+(* Takes a buffer of any color and a yellow buffer of pairs, rearranges
+   elements contained in them, and returns a green buffer and a buffer of pairs
+   of any color.
    The order of elements is preserved. *)
-Equations yellow_prefix_concat {A lvl size1 size2 C}
-  (b1 : buffer A lvl size1 C)
-  (b2 : buffer A (S lvl) size2 yellow) :
-  { '(b1', b2') : buffer A lvl (2 + size1 mod 2) green *
-                  buffer A (S lvl) (Nat.pred (size1 / 2 + size2)) red |
-    buffer_seq b1 ++ buffer_seq b2 =
-    buffer_seq b1' ++ buffer_seq b2' } :=
-yellow_prefix_concat B0 b2 with yellow_pop b2 => {
-  | ? (prodS a b, b3) := ? (B2 a b, b3) };
-yellow_prefix_concat (B1 a) b2 with yellow_pop b2 => {
-  | ? (prodS b c, b3) := ? (B3 a b c, b3) };
-yellow_prefix_concat (B2 a b) b2 := ? (B2 a b, to_red b2);
-yellow_prefix_concat (B3 a b c) b2 := ? (B3 a b c, to_red b2);
-yellow_prefix_concat (B4 a b c d) b2 with yellow_push (prodS c d) b2 => {
-  | ? b3 := ? (B2 a b, b3) };
-yellow_prefix_concat (B5 a b c d e) b2 with yellow_push (prodS d e) b2 => {
-  | ? b3 := ? (B3 a b c, b3) }.
+Equations yellow_prefix_concat {A B}
+  (b1 : buffer A B)
+  (b2 : buffer (A * A) yellow) :
+  { '(b1', b2') : buffer A green * buffer (A * A) red |
+    buffer_seq b1  ++ flattenp (buffer_seq b2) =
+    buffer_seq b1' ++ flattenp (buffer_seq b2') } :=
+yellow_prefix_concat b1 b2 with prefix_decompose b1 => {
+  | ? Underflow opt with yellow_pop b2 => {
+    | ? (ab, b) with prefix23 opt ab => {
+      | ? prefix := ? (prefix, b) } };
+  | ? Ok b := ? (b, to_red b2);
+  | ? Overflow b ab with yellow_push ab b2 => {
+    | ? suffix := ? (b, suffix) } }.
 
-(* Takes a yellow (n+1)-buffer and a n-buffer of any color, rearranges elements
-   contained in them, and returns a buffer of pairs of any color and a green
-   buffer.
+(* Takes a yellow buffer of pairs and a buffer of any color, rearranges
+   elements contained in them, and returns a buffer of pairs of any color and a
+   green buffer.
    The order of elements is preserved. *)
-Equations yellow_suffix_concat {A lvl size1 size2 C}
-  (b1 : buffer A (S lvl) size1 yellow)
-  (b2 : buffer A lvl size2 C) :
-  { '(b1', b2') : buffer A (S lvl) (Nat.pred (size2 / 2 + size1)) red *
-                  buffer A lvl (2 + size2 mod 2) green |
-    buffer_seq b1 ++ buffer_seq b2 =
-    buffer_seq b1' ++ buffer_seq b2' } :=
-yellow_suffix_concat b1 B0 with yellow_eject b1 => {
-  | ? (b3, prodS a b) := ? (b3, B2 a b) };
-yellow_suffix_concat b1 (B1 c) with yellow_eject b1 => {
-  | ? (b3, prodS a b) := ? (b3, B3 a b c) };
-yellow_suffix_concat b1 (B2 a b) := ? (to_red b1, B2 a b);
-yellow_suffix_concat b1 (B3 a b c) := ? (to_red b1, B3 a b c);
-yellow_suffix_concat b1 (B4 a b c d) with yellow_inject b1 (prodS a b) => {
-  | ? b3 := ? (b3, B2 c d) };
-yellow_suffix_concat b1 (B5 a b c d e) with yellow_inject b1 (prodS a b) => {
-  | ? b3 := ? (b3, B3 c d e) }.
-
-(* Pushes an option on a buffer, and returns a green chain. *)
-Equations green_opt_push {A lvl sizeb sizeo}
-    (o : optionN A lvl sizeo) (b : buffer A lvl sizeb green) :
-  { c : chain A lvl (sizeo + sizeb) green |
-    chain_seq c = optionN_seq o ++ buffer_seq b } :=
-green_opt_push NoneN b := ? Ending (to_red b);
-green_opt_push (SomeN a) (B2 b c) := ? Ending (B3 a b c);
-green_opt_push (SomeN a) (B3 b c d) := ? Ending (B4 a b c d).
-
-(* Injects an option on a buffer, and returns a green chain. *)
-Equations green_opt_inject {A lvl sizeb sizeo}
-    (b : buffer A lvl sizeb green) (o : optionN A lvl sizeo) :
-  { c : chain A lvl (sizeo + sizeb) green |
-    chain_seq c = buffer_seq b ++ optionN_seq o } :=
-green_opt_inject b NoneN := ? Ending (to_red b);
-green_opt_inject (B2 a b) (SomeN c) := ? Ending (B3 a b c);
-green_opt_inject (B3 a b c) (SomeN d) := ? Ending (B4 a b c d).
+Equations yellow_suffix_concat {A B}
+  (b1 : buffer (A * A) yellow)
+  (b2 : buffer A B) :
+  { '(b1', b2') : buffer (A * A) red * buffer A green |
+    flattenp (buffer_seq b1) ++ buffer_seq b2 =
+    flattenp (buffer_seq b1') ++ buffer_seq b2' } :=
+yellow_suffix_concat b1 b2 with suffix_decompose b2 => {
+  | ? Underflow opt with yellow_eject b1 => {
+    | ? (b, ab) with suffix23 ab opt => {
+      | ? suffix := ? (b, suffix) } };
+  | ? Ok b := ? (to_red b1, b);
+  | ? Overflow b ab with yellow_inject b1 ab => {
+    | ? prefix := ? (prefix, b) } }.
 
 (* Creates a green chain from 3 options. *)
-Equations chain_of_opt3 {A lvl s1 s2 s3}
-  (o1 : optionN A lvl s1)
-  (o2 : optionN A (S lvl) s2)
-  (o3 : optionN A lvl s3) :
-  { c : chain A lvl (s1 + s2 + s2 + s3) green |
-    chain_seq c = optionN_seq o1 ++ optionN_seq o2 ++ optionN_seq o3 } :=
-chain_of_opt3 NoneN NoneN NoneN := ? Ending B0;
-chain_of_opt3 (SomeN a) NoneN NoneN := ? Ending (B1 a);
-chain_of_opt3 NoneN NoneN (SomeN a) := ? Ending (B1 a);
-chain_of_opt3 (SomeN a) NoneN (SomeN b) := ? Ending (B2 a b);
-chain_of_opt3 NoneN (SomeN (prodS a b)) NoneN := ? Ending (B2 a b);
-chain_of_opt3 (SomeN a) (SomeN (prodS b c)) NoneN := ? Ending (B3 a b c);
-chain_of_opt3 NoneN (SomeN (prodS a b)) (SomeN c) := ? Ending (B3 a b c);
-chain_of_opt3 (SomeN a) (SomeN (prodS b c)) (SomeN d) := ? Ending (B4 a b c d).
+Equations chain_of_opt3 {A}
+  (o1 : option A) (o2 : option (A * A)) (o3 : option A) :
+  { c : chain A green | chain_seq c =
+      option_seq o1 ++ flattenp (option_seq o2) ++ option_seq o3 } :=
+chain_of_opt3 None None None := ? Ending B0;
+chain_of_opt3 (Some a) None None := ? Ending (B1 a);
+chain_of_opt3 None None (Some a) := ? Ending (B1 a);
+chain_of_opt3 (Some a) None (Some b) := ? Ending (B2 a b);
+chain_of_opt3 None (Some (a, b)) None := ? Ending (B2 a b);
+chain_of_opt3 (Some a) (Some (b, c)) None := ? Ending (B3 a b c);
+chain_of_opt3 None (Some (a, b)) (Some c) := ? Ending (B3 a b c);
+chain_of_opt3 (Some a) (Some (b, c)) (Some d) := ? Ending (B4 a b c d).
 
-(* Provided the equality of two natural numbers, translates a chain of size the
-   first into a chain of size the second. *)
-Equations translate {A lvl size1 size2 C} (c : chain A lvl size1 C) :
-  size1 = size2 -> { c' : chain A lvl size2 C | chain_seq c' = chain_seq c } :=
-translate c eq_refl := ? c.
 
-(* Proves that all natural numbers [n] can be writen as [n mod 2] plus 2 times
-   [n / 2]. *)
-Lemma dec_by_2 : forall (n : nat), n mod 2 + n / 2 + n / 2 = n.
-Proof.
-  intro n.
-  assert (n / 2 + n / 2 = 2 * (n / 2)) as H. { lia. }
-  rewrite <-Nat.add_assoc, H, Nat.add_comm.
-  symmetry.
-  apply Nat.div_mod.
-  lia.
-Qed.
-
-(* A hint database of rewrites to be used when trying to automatically resolve
-   obligations on natural numbers generated by [Equations]. *)
-#[export] Hint Rewrite plus_O_n : rnat.
-#[export] Hint Rewrite <-plus_n_O : rnat.
-#[export] Hint Rewrite plus_Sn_m : rnat.
-#[export] Hint Rewrite <-plus_n_Sm : rnat.
-#[export] Hint Rewrite dec_by_2 : rnat.
+(* A new tactic designed for list equalities, applying [flattenp] on them, and
+   simplifying them. *)
+Local Ltac flattenp_eq H :=
+  apply (f_equal flattenp) in H;
+  repeat rewrite flattenp_app in H;
+  cbn in H.
 
 (* Takes a prefix buffer, a child buffer, and a suffix buffer, and rearranges
    all elements contained in these buffers to form a green chain.
    The order of elements is preserved. *)
-Equations make_small {A lvl size1 size2 size3 C1 C2 C3}
-  (b1 : buffer A lvl size1 C1)
-  (b2 : buffer A (S lvl) size2 C2)
-  (b3 : buffer A lvl size3 C3) :
-  { c : chain A lvl (size1 + size2 + size2 + size3) green |
-    chain_seq c = buffer_seq b1 ++ buffer_seq b2 ++ buffer_seq b3 } :=
+Equations make_small {A C1 C2 C3}
+  (b1 : buffer A C1)
+  (b2 : buffer (A * A) C2)
+  (b3 : buffer A C3) :
+  { c : chain A green | chain_seq c =
+      buffer_seq b1 ++ flattenp (buffer_seq b2) ++ buffer_seq b3 } :=
 make_small b1 b2 b3 with prefix_decompose b1, suffix_decompose b3 => {
   | ? Underflow p1, ? Underflow s1 with buffer_unsandwich b2 => {
     | ? Alone opt with chain_of_opt3 p1 opt s1 => { | ? c := ? c };
     | ? Sandwich ab rest cd with prefix23 p1 ab, suffix23 cd s1 => {
-      | ? p, ? s with translate (Chain G (Packet p Hole s) (Ending rest)) _ => {
-        | ? c := ? c } } };
+      | ? p, ? s := ? Chain G (Packet p Hole s) (Ending rest) } };
   | ? Underflow p1, ? Ok s1 with buffer_pop b2 => {
-    | ? None with green_opt_push p1 s1 => {
-      | ? c with translate c _ => { | ? c' := ? c' } };
+    | ? None with p1 => {
+      | None := ? Ending (to_red s1);
+      | Some x with buffer_push x s1 => { | ? c := ? c } };
     | ? Some (cd, rest) with prefix23 p1 cd => {
-      | ? p with translate (Chain G (Packet p Hole s1) (Ending rest)) _ => {
-        | ? c := ? c } } };
+      | ? p := ? Chain G (Packet p Hole s1) (Ending rest) } };
   | ? Underflow p1, ? Overflow s1 ab with suffix_rot b2 ab => {
-    | ? (cd, center) with prefix23 p1 cd => { | ? p
-      with
-        translate (Chain G (Packet p Hole s1) (Ending (to_red center))) _ => {
-          | ? c := ? c } } };
+    | ? (cd, center) with prefix23 p1 cd => {
+      | ? p => ? Chain G (Packet p Hole s1) (Ending (to_red center)) } };
   | ? Ok p1, ? Underflow s1 with buffer_eject b2 => {
-    | ? None with green_opt_inject p1 s1 => {
-      | ? c with translate c _ => { | ? c' := ? c' } };
+    | ? None with s1 => {
+      | None := ? Ending (to_red p1);
+      | Some x with buffer_inject p1 x => { | ? c := ? c } };
     | ? Some (rest, ab) with suffix23 ab s1 => {
-      | ? s with translate (Chain G (Packet p1 Hole s) (Ending rest)) _ => {
-        | ? c := ? c } } };
+      | ? s := ? Chain G (Packet p1 Hole s) (Ending rest) } };
   | ? Ok p1, ? Ok s1 := ? Chain G (Packet p1 Hole s1) (Ending (to_red b2));
   | ? Ok p1, ? Overflow s1 ab with buffer_inject b2 ab => {
-    | ? c2 with translate (Chain G (Packet p1 Hole s1) c2) _ => { | ? c := ? c } };
+    | ? c2 => ? Chain G (Packet p1 Hole s1) c2 };
   | ? Overflow p1 cd, ? Underflow s1 with prefix_rot cd b2 => {
-    | ? (center, ab) with suffix23 ab s1 => { | ? s
-      with
-        translate (Chain G (Packet p1 Hole s) (Ending (to_red center))) _ => {
-          | ? c := ? c } } };
+    | ? (center, ab) with suffix23 ab s1 => {
+      | ? s => ? Chain G (Packet p1 Hole s) (Ending (to_red center)) } };
   | ? Overflow p1 cd, ? Ok s1 with buffer_push cd b2 => {
-    | ? c2
-      with translate (Chain G (Packet p1 Hole s1) c2) _ => { | ? c := ? c } };
+    | ? c2 => ? Chain G (Packet p1 Hole s1) c2 };
   | ? Overflow p1 cd, ? Overflow s1 ab with buffer_halve b2 => {
     | ? (x, rest) with suffix12 cd x => {
-      | ? p :=
-        let c := Chain G (Packet p1 (Packet p Hole (B1 ab)) s1) (Ending rest) in
-        let '? c' := translate c _ in ? c' } } }.
+      | ? p =>
+        ? Chain G (Packet p1 (Packet p Hole (B1 ab)) s1) (Ending rest) } } }.
 Next Obligation.
-  cbn. intros * Hb1 * Hp * Hb2 Hb3 * Hc.
-  rewrite Hc, to_red_seq, Hp.
-  (* Etrange comportement de aac_rewrite, il faut écrire tous
-     les remembers pour qu'il marche. *)
-  remember (prodN_seq ab) as ab_seq.
-  remember (prodN_seq cd) as cd_seq.
-  remember (buffer_seq b2) as b2_seq.
-  remember (buffer_seq center) as center_seq.
+  cbn. intros * Hb1 * Hp * Hb2 Hb3 *.
+  rewrite Hp, to_red_seq.
+  flattenp_eq Hb2.
   aac_rewrite <-Hb2.
   hauto db:rlist.
 Qed.
 Next Obligation.
-  cbn; intros * Hb1 * Hb2 * Hs Hb3 * Hc.
-  rewrite Hc, to_red_seq, Hs.
-  remember (prodN_seq ab) as ab_seq.
-  remember (prodN_seq cd) as cd_seq.
-  remember (buffer_seq b2) as b2_seq.
-  remember (buffer_seq center) as center_seq.
+  cbn. intros * Hb1 * Hb2 * Hs Hb3.
+  rewrite Hs, to_red_seq.
+  flattenp_eq Hb2.
   aac_rewrite <-Hb2.
   hauto db:rlist.
 Qed.
-Next Obligation.
-  intros.
-  autorewrite with rnat.
-  reflexivity.
-Qed.
-
-(* Proves that if a natural number represents the size of a non-red buffer,
-   then it's the successor of another natural number. *)
-Lemma yellow_size {A lvl size g y} (b : buffer A lvl size (Mix g y NoRed)) :
-  exists p, size = S p.
-Proof.
-  dependent destruction b.
-  - exists 0. reflexivity.
-  - exists 1. reflexivity.
-  - exists 2. reflexivity.
-  - exists 3. reflexivity.
-Qed.
-
-(* A tactic to facilitate the use of the previous lemma. *)
-Tactic Notation "yellow_size" hyp(b) "as" ident(H) :=
-  pose (yellow_size b) as H;
-  destruct H as [? H];
-  rewrite H.
 
 (* Makes a red chain green. *)
-Equations green_of_red {A lvl size} (c : chain A lvl size red) :
-  { c' : chain A lvl size green | chain_seq c' = chain_seq c } :=
+Equations green_of_red {A : Type} (c : chain A red) :
+  { c' : chain A green | chain_seq c' = chain_seq c } :=
 green_of_red (Chain R (Packet p1 Hole s1) (Ending b))
   with make_small p1 b s1 => { | ? c' := ? c' };
 green_of_red (Chain R (Packet p1 Hole s1) (Chain G (Packet p2 child s2) c))
   with green_prefix_concat p1 p2, green_suffix_concat s2 s1 => {
   | ? (p1', p2'), ? (s2', s1') :=
-    let c := Chain G (Packet p1' (Packet p2' child s2') s1') c in
-    let '? c' := translate c _ in ? c' };
+    ? Chain G (Packet p1' (Packet p2' child s2') s1') c };
 green_of_red (Chain R (Packet p1 (Packet p2 child s2) s1) c)
   with yellow_prefix_concat p1 (to_yellow p2),
        yellow_suffix_concat (to_yellow s2) s1 => {
   | ? (p1', p2'), ? (s2', s1') :=
-  let c := Chain G (Packet p1' Hole s1') (Chain R (Packet p2' child s2') c) in
-  let '? c' := translate c _ in ? c' }.
+    ? Chain G (Packet p1' Hole s1') (Chain R (Packet p2' child s2') c) }.
 Next Obligation.
-  intros * Hp * Hs * c.
-  yellow_size p2 as Hpsize0. yellow_size s2 as Hssize0.
-  pose (dec_by_2 psize) as Hpsize. rewrite <-Hpsize at 4.
-  pose (dec_by_2 ssize) as Hssize. rewrite <-Hssize at 4.
-  hauto.
-Qed.
-Next Obligation.
-  simpl. intros * Hp * Hs * Hc'.
-  rewrite Hc'.
-  remember (buffer_seq p1) as p1_seq.
-  remember (buffer_seq p2) as p2_seq.
-  remember (buffer_seq p1') as p1'_seq.
-  remember (buffer_seq p2') as p2'_seq.
+  cbn. intros * Hp * Hs *.
+  autorewrite with rlist.
   aac_rewrite <-Hp.
   hauto db:rlist.
 Qed.
 Next Obligation.
-  intros * Hp * Hs * c.
-  yellow_size p2 as Hpsize0. yellow_size s2 as Hssize0.
-  pose (dec_by_2 psize) as Hpsize. rewrite <-Hpsize at 4.
-  pose (dec_by_2 ssize) as Hssize. rewrite <-Hssize at 4.
-  hauto.
-Qed.
-Next Obligation.
-  simpl. intros * Hp * Hs * Hc'.
-  rewrite Hc'.
-  remember (buffer_seq p1) as p1_seq.
-  remember (buffer_seq (to_yellow p2)) as p2_seq.
-  remember (buffer_seq p1') as p1'_seq.
-  remember (buffer_seq p2') as p2'_seq.
+  cbn. intros * Hp * Hs *.
+  autorewrite with rlist.
   aac_rewrite <-Hp.
   hauto db:rlist.
 Qed.
 
 (* Makes a green or red chain green. *)
-Equations ensure_green {A lvl size g r}
-  (cd : chain A lvl size (Mix g NoYellow r)) :
-  { cd' : chain A lvl size green | chain_seq cd' = chain_seq cd } :=
+Equations ensure_green {A g r} (c : chain A (Mix g NoYellow r)) :
+  { c' : chain A green | chain_seq c' = chain_seq c } :=
 ensure_green (Ending b)      := ? Ending b;
 ensure_green (Chain G pkt c) := ? Chain G pkt c;
 ensure_green (Chain R pkt c) := green_of_red (Chain R pkt c).
 
 (* Takes a prefix non-red buffer, a child packet and a suffix non-red buffer,
    and a following green or red chain, and makes a deque out of them. *)
-Equations make_yellow {A lvl ps pkts ss cs size} {gp yp ypkt gs ys gc rc}
-  (p : buffer A 0 ps (Mix gp yp NoRed))
-  (pkt : packet A 1 lvl pkts cs (Mix NoGreen ypkt NoRed))
-  (s : buffer A 0 ss (Mix gs ys NoRed))
-  (c : chain A lvl cs (Mix gc NoYellow rc)) :
-  size = ps + pkts + pkts + ss ->
-  { d : deque A size | deque_seq d =
-    buffer_seq p ++ packet_seq pkt (chain_seq c) ++ buffer_seq s } :=
-make_yellow p1 child s1 c eq_refl with ensure_green c => {
+Equations make_yellow {A B: Type} {g1 y1 y2 g3 y3 g4 r4}
+  (p : buffer A (Mix g1 y1 NoRed))
+  (pkt : packet (A * A) B (Mix NoGreen y2 NoRed))
+  (s : buffer A (Mix g3 y3 NoRed))
+  (c : chain B (Mix g4 NoYellow r4)) :
+  { d : deque A | deque_seq d =
+    buffer_seq p ++ flattenp (packet_seq pkt (chain_seq c)) ++ buffer_seq s } :=
+make_yellow p1 child s1 c with ensure_green c => {
   | ? c' => ? T (Chain Y (Packet (to_yellow p1) child (to_yellow s1)) c') }.
 
 (* Takes a prefix buffer of any color, a child packet and a suffix buffer of
    any color, and a following green chain, and makes a deque out of them. *)
-Equations make_red {A lvl ps pkts ss cs size} {Cp ypkt Cs}
-  (p : buffer A 0 ps Cp)
-  (pkt : packet A 1 lvl pkts cs (Mix NoGreen ypkt NoRed))
-  (s : buffer A 0 ss Cs)
-  (c : chain A lvl cs green) :
-  size = ps + pkts + pkts + ss ->
-  { d : deque A size | deque_seq d =
-    buffer_seq p ++ packet_seq pkt (chain_seq c) ++ buffer_seq s } :=
-make_red p1 child s1 c eq_refl
+Equations make_red {A B: Type} {C1 y2 C3}
+  (p : buffer A C1)
+  (pkt : packet (A * A) B (Mix NoGreen y2 NoRed))
+  (s : buffer A C3)
+  (c : chain B green) :
+  { d : deque A | deque_seq d =
+    buffer_seq p ++ flattenp (packet_seq pkt (chain_seq c)) ++ buffer_seq s } :=
+make_red p1 child s1 c
   with green_of_red (Chain R (Packet (to_red p1) child (to_red s1)) c) => {
     | ? c' => ? T c' }.
 
@@ -938,91 +599,57 @@ make_red p1 child s1 c eq_refl
 (* +------------------------------------------------------------------------+ *)
 
 (* Pushes on a deque. *)
-Equations push {A : Type} {size : nat} (x : A) (d : deque A size) :
-  { d' : deque A (S size) | deque_seq d' = [x] ++ deque_seq d } :=
-push x (T (Ending b)) with buffer_push (prodZ x) b => { | ? b' => ? T b' };
-push x (T (Chain G (Packet p1 child s1) c))
-  with green_push (prodZ x) p1 => {
-    | ? p1' with make_yellow p1' child s1 c eq_refl => { | ? d' => ? d' } };
-push x (T (Chain Y (Packet p1 child s1) c))
-  with yellow_push (prodZ x) p1 => {
-    | ? p1' with make_red p1' child s1 c eq_refl => { | ? d' => ? d' } }.
+Equations push {A : Type} (x : A) (d : deque A) :
+  { d' : deque A | deque_seq d' = [x] ++ deque_seq d } :=
+push x (T (Ending b)) with buffer_push x b => { | ? b' => ? T b' };
+push x (T (Chain G (Packet p1 child s1) c)) with green_push x p1 => {
+  | ? p1' with make_yellow p1' child s1 c => {
+    | ? d' => ? d' } };
+push x (T (Chain Y (Packet p1 child s1) c)) with yellow_push x p1 => {
+  | ? p1' with make_red p1' child s1 c => {
+    | ? d' => ? d' } }.
 
 (* Injects on a deque. *)
-Equations inject {A : Type} {size : nat} (d : deque A size) (x : A) :
-  { d' : deque A (S size) | deque_seq d' = deque_seq d ++ [x] } :=
-inject (T (Ending b)) x with buffer_inject b (prodZ x) => { | ? b' => ? T b' };
-inject (T (Chain G (Packet p1 child s1) c)) x
-  with green_inject s1 (prodZ x) => {
-    | ? s1' with make_yellow p1 child s1' c _ => { | ? d' => ? d' } };
-inject (T (Chain Y (Packet p1 child s1) c)) x
-  with yellow_inject s1 (prodZ x) => {
-    | ? s1' with make_red p1 child s1' c _ => { | ? d' => ? d' } }.
+Equations inject {A : Type} (d : deque A) (x : A) :
+  { d' : deque A | deque_seq d' = deque_seq d ++ [x] } :=
+inject (T (Ending b)) x with buffer_inject b x => { | ? b' => ? T b' };
+inject (T (Chain G (Packet p1 child s1) c)) x with green_inject s1 x => {
+  | ? s1' with make_yellow p1 child s1' c => {
+    | ? d' => ? d' } };
+inject (T (Chain Y (Packet p1 child s1) c)) x with yellow_inject s1 x => {
+  | ? s1' with make_red p1 child s1' c => {
+    | ? d' => ? d' } }.
 
 (* Pops off a deque. *)
-Equations option_pop {A : Type} {size : nat} (d : deque A size) :
-  { o : option (A * deque A (Nat.pred size)) |
-    match o with
-    | None => deque_seq d = [] /\ size = 0
-    | Some (x, d') => deque_seq d = [x] ++ deque_seq d'
-    end } :=
-option_pop (T (Ending b)) with buffer_pop b => {
+Equations pop {A : Type} (d : deque A) :
+  { o : option (A * deque A) |
+    deque_seq d = match o with
+                  | None => []
+                  | Some (x, d') => [x] ++ deque_seq d'
+                  end } :=
+pop (T (Ending b)) with buffer_pop b => {
   | ? None := ? None;
-  | ? Some (prodZ x, b') := ? Some (x, T (Ending b')) };
-option_pop (T (Chain G (Packet p1 child s1) c)) with green_pop p1 => {
-  | ? (prodZ x, p1') with make_yellow p1' child s1 c _ => {
+  | ? Some (x, b') := ? Some (x, T (Ending b')) };
+pop (T (Chain G (Packet p1 child s1) c)) with green_pop p1 => {
+  | ? (x, p1') with make_yellow p1' child s1 c => {
     | ? d' => ? Some (x, d') } };
-option_pop (T (Chain Y (Packet p1 child s1) c)) with yellow_pop p1 => {
-  | ? (prodZ x, p1') with make_red p1' child s1 c _ => {
+pop (T (Chain Y (Packet p1 child s1) c)) with yellow_pop p1 => {
+  | ? (x, p1') with make_red p1' child s1 c => {
     | ? d' => ? Some (x, d') } }.
-Next Obligation.
-  intros * Hp1 child s1 c.
-  yellow_size p1 as H.
-  hauto.
-Qed.
-Next Obligation.
-  intros * Hp1 child s1 c.
-  yellow_size p1 as H.
-  hauto.
-Qed.
-
-(* Pops off a non-empty deque. *)
-Equations pop {A : Type} {size : nat} (d : deque A (S size)) :
-  { '(x, d') : A * deque A size | deque_seq d = [x] ++ deque_seq d' } :=
-pop d with option_pop d => {
-  | ? None := _;
-  | ? Some (x, d') := ? (x, d') }.
 
 (* Ejects off a deque. *)
-Equations option_eject {A : Type} {size : nat} (d : deque A size) :
-  { o : option (deque A (Nat.pred size) * A) |
-    match o with
-    | None => deque_seq d = [] /\ size = 0
-    | Some (d', x) => deque_seq d = deque_seq d' ++ [x]
-    end } :=
-option_eject (T (Ending b)) with buffer_eject b => {
+Equations eject {A : Type} (d : deque A) :
+  { o : option (deque A * A) |
+    deque_seq d = match o with
+                  | None => []
+                  | Some (d', x) => deque_seq d' ++ [x]
+                  end } :=
+eject (T (Ending b)) with buffer_eject b => {
   | ? None := ? None;
-  | ? Some (b', prodZ x) := ? Some (T (Ending b'), x) };
-option_eject (T (Chain G (Packet p1 child s1) c)) with green_eject s1 => {
-  | ? (s1',prodZ  x) with make_yellow p1 child s1' c _ => {
+  | ? Some (b', x) := ? Some (T (Ending b'), x) };
+eject (T (Chain G (Packet p1 child s1) c)) with green_eject s1 => {
+  | ? (s1', x) with make_yellow p1 child s1' c => {
     | ? d' => ? Some (d', x) } };
-option_eject (T (Chain Y (Packet p1 child s1) c)) with yellow_eject s1 => {
-  | ? (s1', prodZ x) with make_red p1 child s1' c _ => {
+eject (T (Chain Y (Packet p1 child s1) c)) with yellow_eject s1 => {
+  | ? (s1', x) with make_red p1 child s1' c => {
     | ? d' => ? Some (d', x) } }.
-Next Obligation.
-  intros * p1 child * Hs1 c.
-  yellow_size s1 as H.
-  hauto.
-Qed.
-Next Obligation.
-  intros * p1 child * Hs1 c.
-  yellow_size s1 as H.
-  hauto.
-Qed.
-
-(* Ejects off a non-empty deque. *)
-Equations eject {A : Type} {size : nat} (d : deque A (S size)) :
-  { '(d', x) : deque A size * A | deque_seq d = deque_seq d' ++ [x] } :=
-eject d with option_eject d => {
-  | ? None := _;
-  | ? Some (d', x) := ? (d', x) }.
