Color/GYOR.v
@@ -25,7 +25,7 @@ Notation orange := (Mix NoGreen NoYellow SomeOrange NoRed).
 Notation red := (Mix NoGreen NoYellow NoOrange SomeRed).
 Notation uncolored := (Mix NoGreen NoYellow NoOrange NoRed).
 
-(* An instance of [UIP] for colors is needed in Deque/core.v. *)
+(* An instance of [UIP] for colors is needed in Cadeque/core.v. *)
 Instance UIP_color : UIP color.
 Proof.
   intros C1 C2 p q.
